WIP tactic for higher-order rewriting; need to enable the specialization argument

code/meta/Example.fst
@@ -1,5 +1,7 @@
 module Example
 
+module I = Interface
+
 open FStar.Mul
 
 #set-options "--print_bound_var_types"
@@ -10,8 +12,8 @@ open FStar.Mul
   times_sixteen'_inline
 ] (MetaInterface.specialize [ `Client.times_sixteen; `Client.times_sixteen' ])
 
-let add: Interface.add_st = fun x y -> x + y
-let mul: Interface.mul_st = fun x y -> x * y
+let add: I.add_st I.W32 = FStar.UInt32.add_mod
+let mul: I.mul_st I.W32 = FStar.UInt32.mul_mod
 let times_four = times_four_inline add
 let times_sixteen = times_sixteen_inline times_four
 let times_sixteen' = times_sixteen'_inline times_four mul
