code/meta/Client.fst
@@ -5,21 +5,24 @@ module Client
 module I = Interface
 
 [@ MetaAttribute.inline_ ]
-let times_two (x: int) =
+let times_two #w (x: I.word w) =
   I.add x x
 
 [@ MetaAttribute.specialize ]
-let times_four (x: int) =
+let times_four #w (x: I.word w) =
   times_two (times_two x)
 
 [@ MetaAttribute.inline_ ]
-let times_four' (x: int) =
-  I.mul 4 x
+let four #w: I.word w = if w = I.W32 then 4ul else 4UL
+
+[@ MetaAttribute.inline_ ]
+let times_four' #w (x: I.word w) =
+  I.mul four x
 
 [@ MetaAttribute.specialize ]
-let times_sixteen (x: int) =
+let times_sixteen #w (x: I.word w) =
   times_four (times_four x)
 
 [@ MetaAttribute.specialize ]
-let times_sixteen' (x: int) =
+let times_sixteen' #w (x: I.word w) =
   times_four (times_four' x)
